Better illustration of positivity check

Magic.v
@@ -1,8 +1,50 @@
-Unset Guard Checking.
+Require Import String.
 
+#[bypass_check(guard)]
 Fixpoint magic (x : nat) : False := magic x.
 
 Goal False.
-  apply magic. exact 0.
-Qed.
+  exact (magic 0).
+Abort.
+
+#[bypass_check(positivity)]
+Inductive D := Fix (f : D -> D).
+
+Fixpoint magic_ind (d : D) : False :=
+  match d with
+  | Fix f => magic_ind (f d)
+  end.
+
+Fixpoint inhab (d : D) : D :=
+  match d with
+  | Fix f => Fix (fun d => inhab (f d))
+  end.
+
+Goal False.
+  exact (magic_ind (Fix inhab)).
+Abort.
+
+(* test locality of bypass_check *)
+Definition var := string.
+
+Inductive tm := Var (x : var) | Lam (x : var) (e : tm) | App (e1 e2 : tm).
+
+Inductive value := Clos (x : var) (e : tm) (σ : var -> option value).
+
+Definition env := var -> option value.
+
+Fixpoint eval (e : tm) (σ : env) {struct e} : option value.
+Proof.
+  exact (
+  match e with
+  | Var x => σ x
+  | Lam x e => Some (Clos x e σ)
+  | App e1 e2 =>
+    match eval e1 σ, eval e2 σ with
+    | Some (Clos x e σ), Some v =>
+      eval e (fun x' => if x =? x' then Some v else σ x')%string
+    | _, _ => None
+    end
+  end).
+Fail Qed.
 
